updates to make everything compile again (or comment out), so that the compiler target can be added back to CI

compiler/src/ExprImp.v
@@ -1,3 +1,4 @@
+Require Import Coq.ZArith.ZArith.
 Require Import Coq.Lists.List. Import ListNotations.
 Require Import Coq.Program.Tactics.
 Require Import bbv.DepEqNat.
@@ -9,10 +10,12 @@ Require Export bedrock2.Semantics.
 Require Import coqutil.Macros.unique.
 Require Import compiler.util.Common.
 Require Import compiler.util.Tactics.
-Require Import compiler.Op.
 Require Import coqutil.Decidable.
-Require Import compiler.Memory.
-Require Import bedrock2.Semantics. (* TODO: this should be in bedrock2.Semantics *)
+Require Import coqutil.Datatypes.PropSet.
+Require Import riscv.util.ListLib.
+
+
+Open Scope Z_scope.
 
 Local Notation "' x <- a ; f" :=
   (match (a: option _) with
@@ -25,53 +28,39 @@ Section ExprImp1.
 
   Context {p : unique! Semantics.parameters}.
 
-  Notation mword := (@Semantics.word p).
-  Context {MW: MachineWidth mword}.
-
-  Notation var := (@Syntax.varname (@Semantics.syntax p)).
-  Notation func := (@Syntax.funname (@Semantics.syntax p)).
-
-  Context {stateMap: MapFunctions varname (mword)}.
-  (*Notation state := (map varname mword).*)
-  Context {varnameset: SetFunctions varname}.
-  Notation vars := (set varname).
+  Notation var := (@Syntax.varname (@Semantics.syntax p)) (only parsing).
+  Notation func := (@Syntax.funname (@Semantics.syntax p)) (only parsing).
+  Notation vars := (var -> Prop).
 
   (*Hypothesis actname_empty: Syntax.actname = Empty_set.*)
   Local Notation actname := Syntax.actname.
 
-  Context {Event: Type}.
-  Local Notation trace := (list Event).
-
-  Ltac state_calc := map_solver (@varname (@Semantics.syntax p)) (@Semantics.word p).
-  Ltac set_solver := set_solver_generic (@varname (@Semantics.syntax p)).
+  Ltac set_solver := set_solver_generic (@Syntax.varname (@Semantics.syntax p)).
+  Context {word_ok: word.ok word}. (* TODO which param record? *)
 
   Section WithEnv.
-    Context {funcMap: MapFunctions funcname (list varname * list varname * cmd)}.
-    Notation env := (map funcname (list varname * list varname * cmd)).
     Context (e: env).
-
-    Notation mem := (map mword Semantics.byte).
 
     Fixpoint eval_cmd(f: nat)(st: locals)(m: mem)(s: cmd): option (locals * mem) :=
       match f with
-      | 0 => None (* out of fuel *)
+      | O => None (* out of fuel *)
       | S f => match s with
         | cmd.store aSize a v =>
             'Some a <- eval_expr m st a;
             'Some v <- eval_expr m st v;
-            'Some m <- Semantics.store (bytes_per aSize) m a v;
+            'Some m <- store aSize m a v;
             Some (st, m)
         | cmd.set x e =>
             'Some v <- eval_expr m st e;
-            Some (put st x v, m)
+            Some (map.put st x v, m)
         | cmd.unset x =>
-            Some (remove_key st x, m)
+            Some (map.remove st x, m)
         | cmd.cond cond bThen bElse =>
             'Some v <- eval_expr m st cond;
-            eval_cmd f st m (if reg_eqb v (ZToReg 0) then bElse else bThen)
+            eval_cmd f st m (if word.eqb v (word.of_Z 0) then bElse else bThen)
         | cmd.while cond body =>
             'Some v <- eval_expr m st cond;
-            if reg_eqb v (ZToReg 0) then Some (st, m) else
+            if word.eqb v (word.of_Z 0) then Some (st, m) else
               'Some (st, m) <- eval_cmd f st m body;
               eval_cmd f st m (cmd.while cond body)
         | cmd.seq s1 s2 =>
@@ -79,48 +68,74 @@ Section ExprImp1.
             eval_cmd f st m s2
         | cmd.skip => Some (st, m)
         | cmd.call binds fname args =>
-          'Some (params, rets, fbody) <- get e fname;
+          'Some (params, rets, fbody) <- map.get e fname;
           'Some argvs <- option_all (List.map (eval_expr m st) args);
-          'Some st0 <- putmany params argvs empty_map;
+          'Some st0 <- map.putmany_of_list params argvs map.empty;
           'Some (st1, m') <- eval_cmd f st0 m fbody;
-          'Some retvs <- option_all (List.map (get st1) rets);
-          'Some st' <- putmany binds retvs st;
+          'Some retvs <- option_all (List.map (map.get st1) rets);
+          'Some st' <- map.putmany_of_list binds retvs st;
           Some (st', m')
         | cmd.interact _ _ _ => None (* unsupported *)
         end
       end.
 
-    Fixpoint expr_size(e: expr): nat :=
+    Fixpoint expr_size(e: expr): Z :=
       match e with
       | expr.literal _ => 8
-      | expr.load _ e => S (expr_size e)
+      | expr.load _ e => expr_size e + 1
       | expr.var _ => 1
-      | expr.op op e1 e2 => S (S (expr_size e1 + expr_size e2))
+      | expr.op op e1 e2 => expr_size e1 + expr_size e2 + 2
       end.
 
-    Fixpoint cmd_size(s: cmd): nat :=
+    Lemma expr_size_pos: forall exp, expr_size exp > 0.
+    Proof.
+      induction exp; simpl; try omega.
+    Qed.
+
+    Fixpoint cmd_size(s: cmd): Z :=
       match s with
-      | cmd.store _ a v => S (expr_size a + expr_size v)
-      | cmd.set x e => S (expr_size e)
-      | cmd.cond cond bThen bElse => S (expr_size cond + cmd_size bThen + cmd_size bElse)
-      | cmd.while cond body => S (expr_size cond + cmd_size body)
-      | cmd.seq s1 s2 => S (cmd_size s1 + cmd_size s2)
+      | cmd.store _ a v => expr_size a + expr_size v + 1
+      | cmd.set x e => expr_size e + 1
+      | cmd.cond cond bThen bElse => expr_size cond + cmd_size bThen + cmd_size bElse + 1
+      | cmd.while cond body => expr_size cond + cmd_size body + 1
+      | cmd.seq s1 s2 => cmd_size s1 + cmd_size s2 + 1
       | cmd.skip | cmd.unset _ => 1
       | cmd.call binds f args =>
-          S (length binds + length args + List.fold_right Nat.add O (List.map expr_size args))
-      | cmd.interact _ _ exprs => fold_left (fun res e => res + expr_size e) exprs 0
+          Zlength binds + Zlength args + List.fold_right Z.add 0 (List.map expr_size args) + 1
+      | cmd.interact _ _ exprs => fold_right (fun e res => res + expr_size e) 0 exprs
                                   + 7 (* randomly chosen max allowed number of instructions
                                          one interaction can be compiled to, TODO parametrize
                                          over this *)
       end.
+
+    Lemma cmd_size_pos: forall s, cmd_size s > 0.
+    Proof.
+      induction s; simpl;
+      repeat match goal with
+      | e: expr |- _ => unique pose proof (expr_size_pos e)
+      | l: list _ |- _ => unique pose proof (Zlength_nonneg l)
+      end;
+      try omega;
+      induction args;
+      simpl;
+      rewrite? Zlength_nil in *;
+      try omega;
+      rewrite? Zlength_cons in *;
+      repeat match goal with
+      | e: expr |- _ => unique pose proof (expr_size_pos e)
+      | l: list _ |- _ => unique pose proof (Zlength_nonneg l)
+      | A: _ -> _, B: _ |- _ => specialize (A B)
+      end;
+      try omega.
+    Qed.
 
     Local Ltac inversion_lemma :=
       intros;
       simpl in *;
       repeat (destruct_one_match_hyp; try discriminate);
       repeat match goal with
-             | E: reg_eqb _ _ = true  |- _ => apply reg_eqb_true  in E
-             | E: reg_eqb _ _ = false |- _ => apply reg_eqb_false in E
+             | E: _ _ _ = true  |- _ => apply word.eqb_true  in E
+             | E: _ _ _ = false |- _ => apply word.eqb_false in E
              end;
       inversionss;
       eauto 16.
@@ -129,35 +144,35 @@ Section ExprImp1.
       eval_cmd (S fuel) initialSt initialM (cmd.store aSize a v) = Some final ->
       exists av vv finalM, eval_expr initialM initialSt a = Some av /\
                            eval_expr initialM initialSt v = Some vv /\
-                           Semantics.store (bytes_per aSize) initialM av vv = Some finalM /\
+                           store aSize initialM av vv = Some finalM /\
                            final = (initialSt, finalM).
     Proof. inversion_lemma. Qed.
 
     Lemma invert_eval_set: forall f st1 m1 p2 x e,
       eval_cmd (S f) st1 m1 (cmd.set x e) = Some p2 ->
-      exists v, eval_expr m1 st1 e = Some v /\ p2 = (put st1 x v, m1).
+      exists v, eval_expr m1 st1 e = Some v /\ p2 = (map.put st1 x v, m1).
     Proof. inversion_lemma. Qed.
 
     Lemma invert_eval_unset: forall f st1 m1 p2 x,
       eval_cmd (S f) st1 m1 (cmd.unset x) = Some p2 ->
-      p2 = (remove_key st1 x, m1).
+      p2 = (map.remove st1 x, m1).
     Proof. inversion_lemma. Qed.
 
     Lemma invert_eval_cond: forall f st1 m1 p2 cond bThen bElse,
       eval_cmd (S f) st1 m1 (cmd.cond cond bThen bElse) = Some p2 ->
       exists cv,
         eval_expr m1 st1 cond = Some cv /\
-        (cv <> ZToReg 0 /\ eval_cmd f st1 m1 bThen = Some p2 \/
-         cv = ZToReg 0  /\ eval_cmd f st1 m1 bElse = Some p2).
+        (cv <> word.of_Z 0 /\ eval_cmd f st1 m1 bThen = Some p2 \/
+         cv = word.of_Z 0  /\ eval_cmd f st1 m1 bElse = Some p2).
     Proof. inversion_lemma. Qed.
 
     Lemma invert_eval_while: forall st1 m1 p3 f cond body,
       eval_cmd (S f) st1 m1 (cmd.while cond body) = Some p3 ->
       exists cv,
         eval_expr m1 st1 cond = Some cv /\
-        (cv <> ZToReg 0 /\ (exists st2 m2, eval_cmd f st1 m1 body = Some (st2, m2) /\
+        (cv <> word.of_Z 0 /\ (exists st2 m2, eval_cmd f st1 m1 body = Some (st2, m2) /\
                                      eval_cmd f st2 m2 (cmd.while cond body) = Some p3) \/
-         cv = ZToReg 0 /\ p3 = (st1, m1)).
+         cv = word.of_Z 0 /\ p3 = (st1, m1)).
     Proof. inversion_lemma. Qed.
 
     Lemma invert_eval_seq: forall st1 m1 p3 f s1 s2,
@@ -173,12 +188,12 @@ Section ExprImp1.
     Lemma invert_eval_call : forall st m1 p2 f binds fname args,
       eval_cmd (S f) st m1 (cmd.call binds fname args) = Some p2 ->
       exists params rets fbody argvs st0 st1 m' retvs st',
-        get e fname = Some (params, rets, fbody) /\
+        map.get e fname = Some (params, rets, fbody) /\
         option_all (List.map (eval_expr m1 st) args) = Some argvs /\
-        putmany params argvs empty_map = Some st0 /\
+        map.putmany_of_list params argvs map.empty = Some st0 /\
         eval_cmd f st0 m1 fbody = Some (st1, m') /\
-        option_all (List.map (get st1) rets) = Some retvs /\
-        putmany binds retvs st = Some st' /\
+        option_all (List.map (map.get st1) rets) = Some retvs /\
+        map.putmany_of_list binds retvs st = Some st' /\
         p2 = (st', m').
     Proof. inversion_lemma. Qed.
 
@@ -190,7 +205,7 @@ Section ExprImp1.
   End WithEnv.
 
   (* Returns a list to make it obvious that it's a finite set. *)
-  Fixpoint allVars_expr(e: expr): list varname :=
+  Fixpoint allVars_expr(e: expr): list var :=
     match e with
     | expr.literal v => []
     | expr.var x => [x]
@@ -198,7 +213,7 @@ Section ExprImp1.
     | expr.op op e1 e2 => (allVars_expr e1) ++ (allVars_expr e2)
     end.
 
-  Fixpoint allVars_cmd(s: cmd): list varname :=
+  Fixpoint allVars_cmd(s: cmd): list var :=
     match s with
     | cmd.store _ a e => (allVars_expr a) ++ (allVars_expr e)
     | cmd.set v e => v :: allVars_expr e
@@ -234,24 +249,18 @@ Section ExprImp1.
     - set_solver.
     - set_solver.
     - set_solver.
-    - exfalso. eapply empty_set_spec. eassumption.
-    - apply union_spec in H.
-      apply in_or_app. right. apply in_or_app.
-      destruct H as [H|H]; auto.
-    - apply union_spec in H.
-      apply in_or_app.
-      destruct H as [H|H]; auto.
+    - set_solver.
+    - set_solver.
+      + apply in_or_app. right. apply in_or_app. left. assumption.
+      + apply in_or_app. right. apply in_or_app. right. assumption.
+    - set_solver; apply in_or_app; auto.
     - apply in_or_app. right. auto.
     - generalize dependent binds; induction binds; intros H; cbn in *.
-      + apply empty_set_spec in H; destruct H.
-      + apply union_spec in H; destruct H.
-        * left. apply singleton_set_spec in H. auto.
-        * right. auto.
+      + contradiction.
+      + destruct H; auto.
     - generalize dependent binds; induction binds; intros H; cbn in *.
-      + apply empty_set_spec in H; destruct H.
-      + apply union_spec in H; destruct H.
-        * left. apply singleton_set_spec in H. auto.
-        * right. auto.
+      + contradiction.
+      + destruct H; auto.
   Qed.
 
 End ExprImp1.
@@ -290,35 +299,23 @@ Section ExprImp2.
 
   Context {p : unique! Semantics.parameters}.
 
-  Notation mword := (@Semantics.word p).
-  Context {MW: MachineWidth mword}.
-
-  Notation var := (@Syntax.varname (@Semantics.syntax p)).
-  Notation func := (@Syntax.funname (@Semantics.syntax p)).
-
-  Context {stateMap: MapFunctions varname (mword)}.
-  (*Notation state := (map varname mword).*)
-  Context {varnameset: SetFunctions varname}.
-  Notation vars := (set varname).
+  Notation var := (@Syntax.varname (@Semantics.syntax p)) (only parsing).
+  Notation func := (@Syntax.funname (@Semantics.syntax p)) (only parsing).
+  Notation vars := (var -> Prop).
 
   (*Hypothesis actname_empty: Syntax.actname = Empty_set.*)
   Local Notation actname := Syntax.actname.
 
-  Context {Event: Type}.
-  Local Notation trace := (list Event).
+  Context {word_ok: word.ok word}. (* TODO which param record? *)
+  Context {locals_ok: map.ok locals}.
+  Context {varname_dec: DecidableEq Syntax.varname}.
 
-  Ltac state_calc := map_solver (@varname (@Semantics.syntax p)) (@Semantics.word p).
-  Ltac set_solver := set_solver_generic (@varname (@Semantics.syntax p)).
-
-  (* TODO this one should be wrapped somewhere *)
-  Context {varname_eq_dec: DecidableEq varname}.
-
-  Context {funcMap: MapFunctions funcname (list varname * list varname * cmd)}.
-  Notation env := (map funcname (list varname * list varname * cmd)).
+  Ltac state_calc := map_solver locals_ok.
+  Ltac set_solver := set_solver_generic (@Syntax.varname (@Semantics.syntax p)).
 
   Lemma modVarsSound: forall (e: env) fuel s initialS initialM finalS finalM,
     eval_cmd e fuel initialS initialM s = Some (finalS, finalM) ->
-    only_differ initialS (modVars s) finalS.
+    map.only_differ initialS (modVars s) finalS.
   Proof.
     induction fuel; introv Ev.
     - discriminate.
@@ -331,7 +328,6 @@ Section ExprImp2.
           ensure_new IH'
       end;
       state_calc;
-      (rewrite ?get_remove_key; state_calc);
       refine (only_differ_putmany _ _ _ _ _ _); eassumption.
   Qed.
 
