compiler/src/Basic32Semantics.v
@@ -2,22 +2,30 @@ Require Import Coq.ZArith.ZArith.
 Require Import bedrock2.Syntax bedrock2.Semantics.
 Require Import coqutil.Map.SortedList.
 Require Import bedrock2.ZNamesSyntax.
-Require Import compiler.Op.
-Require Import riscv.MachineWidth32.
+Require Import riscv.Words32Naive.
+Require Import riscv.DefaultMemImpl32.
+Require Import compiler.examples.Empty_set_keyed_map.
+Require Import compiler.examples.Z_keyed_map.
+Require Import bedrock2.Basic_bopnames.
 
 Definition TODO{T: Type}: T. Admitted.
 
+Instance Basic32Syntax: bedrock2.Syntax.parameters := {|
+  Syntax.varname := Z;
+  Syntax.funname := Empty_set;
+  Syntax.actname := Empty_set;
+  Syntax.bopname := Basic_bopnames.bopname;
+|}.
+
 Instance Basic32Semantics: bedrock2.Semantics.parameters. unshelve refine {|
-  Semantics.syntax := {|
-    Syntax.varname := Z;
-    Syntax.funname := Empty_set;
-    Syntax.actname := Empty_set;
-    Syntax.bopname := bopname;
-  |};
-  Semantics.interp_binop bop := eval_binop bop;
+  Semantics.syntax := Basic32Syntax;
+  Semantics.width := 32;
+  Semantics.word := word32;
+  Semantics.byte := word8;
+  Semantics.locals := _;
+  Semantics.env := Empty_set_keyed_map _;
+  Semantics.mem := Mem;  Semantics.interp_binop := interp_binop;
 |}.
 Proof.
-  all: try exact _.
-  (* all other fields are unused: *)
   all: apply TODO.
 Defined.
