compiler/src/FlatToRiscv64Specifics.v
@@ -5,7 +5,10 @@ Require Import riscv.Utility.
 Require Import compiler.FlatToRiscvBitWidthSpecifics.
 Require Import riscv.Memory.
 
-Instance FlatToRiscv64Specifics{byte: word 8}{word64: word 64}{Mem: map.map word64 byte}
+Instance FlatToRiscv64Specifics
+         {byte: Word.Interface.word 8}
+         {word64: Word.Interface.word 64}
+         {Mem: map.map word64 byte}
   : FlatToRiscvBitWidthSpecifics word64  := {|
 
   BitWidth := BW64;
