compiler/src/examples/EditDistExample.v
@@ -1,3 +1,4 @@
+Require Import Coq.ZArith.ZArith.
 Require Import compiler.ExprImp.
 Require Import riscv.util.BitWidths.
 Require Import compiler.util.Common.
@@ -14,7 +15,6 @@ Require Import compiler.examples.Fibonacci.
 Require Import Coq.Strings.String.
 Require Import Coq.Strings.Ascii.
 Require Import compiler.NameGen.
-Require Import riscv.MachineWidth32.
 Require Import riscv.util.BitWidth32.
 
 
