compiler/src/examples/Empty_set_keyed_map.v
@@ -1,0 +1,16 @@
+Require Import coqutil.Map.Interface.
+Require Import coqutil.Map.SortedList.
+
+Instance Empty_set_strictorder: SortedList.parameters.strict_order
+                                  (fun (e1 e2: Empty_set) => false).
+Proof.
+  constructor; intros; match goal with x: Empty_set |- _ => destruct x end.
+Qed.
+
+Instance Empty_set_keyed_map_params(V: Type): SortedList.parameters := {|
+  parameters.key := Empty_set;
+  parameters.value := V;
+  parameters.ltb e1 e2 := false;
+|}.
+Instance Empty_set_keyed_map(V: Type): map.map Empty_set V :=
+  SortedList.map (Empty_set_keyed_map_params V) Empty_set_strictorder.
