compiler/src/examples/TestFlatImp.v
@@ -3,7 +3,6 @@ Require Import riscv.util.Word.
 Require Import riscv.util.BitWidths.
 Require Import compiler.util.Common.
 Require Import compiler.util.Tactics.
-Require Import compiler.Op.
 Require Import coqutil.Decidable.
 Require Import riscv.util.BitWidth32.
 Require Import coqutil.Map.SortedList.
@@ -11,6 +10,9 @@ Require Import compiler.util.List_Set.
 Require Import compiler.FlatImp.
 Require Import riscv.Words32Naive.
 Require Import riscv.DefaultMemImpl32.
+Require Import compiler.examples.Empty_set_keyed_map.
+Require Import compiler.examples.Z_keyed_map.
+Require Import bedrock2.Basic_bopnames.
 
 
 Definition var: Set := Z. (* only inside this test module *)
@@ -55,41 +57,12 @@ Example fib(n: Z): stmt  :=
               (SOp _n bopname.sub _n _one)))))
   )))).
 
-Instance Zltb_strictorder: SortedList.parameters.strict_order Z.ltb.
-Proof.
-  constructor; intros; rewrite ?Z.ltb_lt, ?Z.ltb_ge, ?Z.ltb_irrefl in *;
-    reflexivity || lia.
-Qed.
-
-Instance Zkeyed_map_params(V: Type): SortedList.parameters := {|
-  parameters.key := Z;
-  parameters.value := V;
-  parameters.ltb := Z.ltb;
-|}.
-
-Instance Zkeyed_map(V: Type): map.map Z V :=
-  SortedList.map (Zkeyed_map_params V) Zltb_strictorder.
-
-Instance Empty_set_strictorder: SortedList.parameters.strict_order
-                                  (fun (e1 e2: Empty_set) => false).
-Proof.
-  constructor; intros; match goal with x: Empty_set |- _ => destruct x end.
-Qed.
-
-Instance Empty_set_keyed_map_params(V: Type): SortedList.parameters := {|
-  parameters.key := Empty_set;
-  parameters.value := V;
-  parameters.ltb e1 e2 := false;
-|}.
-Instance Empty_set_keyed_map(V: Type): map.map Empty_set V :=
-  SortedList.map (Empty_set_keyed_map_params V) Empty_set_strictorder.
-
-Instance Registers: map.map varname word32 := Zkeyed_map word32.
+Set Refine Instance Mode.
 
 Instance myFlatImpParams: FlatImp.parameters := {|
   FlatImp.bopname_params := myparams;
   FlatImp.W := Words32Naive;
-  FlatImp.locals := Registers;
+  FlatImp.locals := Zkeyed_map word32;
   FlatImp.env := Empty_set_keyed_map _;
   FlatImp.mem := Mem;
   FlatImp.locals_ok := @SortedList.map_ok (Zkeyed_map_params _) _;
@@ -97,7 +70,7 @@ Instance myFlatImpParams: FlatImp.parameters := {|
   FlatImp.mem_ok := @SortedList.map_ok DefaultMemImpl32.params _;
   FlatImp.ext_spec t m action args outcome := False;
   FlatImp.max_ext_call_code_size name := 0%Z;
-|}.
+|}. cbv. intros. discriminate. Defined.
 
 Definition eval_stmt_test fuel initialSt := eval_stmt map.empty fuel initialSt map.empty.
 
