compiler/src/examples/Z_keyed_map.v
@@ -1,0 +1,19 @@
+Require Import Coq.ZArith.ZArith.
+Require Import Coq.micromega.Lia.
+Require Import coqutil.Map.Interface.
+Require Import coqutil.Map.SortedList.
+
+Instance Zltb_strictorder: SortedList.parameters.strict_order Z.ltb.
+Proof.
+  constructor; intros; rewrite ?Z.ltb_lt, ?Z.ltb_ge, ?Z.ltb_irrefl in *;
+    reflexivity || lia.
+Qed.
+
+Instance Zkeyed_map_params(V: Type): SortedList.parameters := {|
+  parameters.key := Z;
+  parameters.value := V;
+  parameters.ltb := Z.ltb;
+|}.
+
+Instance Zkeyed_map(V: Type): map.map Z V :=
+  SortedList.map (Zkeyed_map_params V) Zltb_strictorder.
