compiler/src/util/Common.v
@@ -4,7 +4,6 @@ Require Export coqutil.Map.Interface coqutil.Map.Properties coqutil.Map.Solver.
 Require Export coqutil.Word.Interface coqutil.Word.Properties.
 Require Export coqutil.Decidable.
 Require Export compiler.util.Tactics.
-Require Export compiler.util.Set.
 Require Export lib.fiat_crypto_tactics.UniquePose.
 
 
